---
title: "STAT-S632"
subtitle: 'Assignment 0'
author: "John Koo"
output: pdf_document
# output: html_document
urlcolor: blue
header-includes:
- \usepackage{float}
---

```{r setup, include = FALSE}
knitr::opts_chunk$set(echo = TRUE, 
                      comment = NA, 
                      warning = FALSE, 
                      message = FALSE, 
                      fig.pos = 'H', 
                      fig.align = 'center', 
                      fig.height = 5, 
                      fig.width = 5)
options(xtable.comment = FALSE, 
        xtable.table.placement = 'H')
```

# Problem 1

Bias is defined as:

$$bias(\hat{y}|x) = 
\big(x_{1i}^T (X_1^T X_1)^{-1} X_1^T X_2^T - x_{2i}^T \big) \beta_2$$

Then:

$$\sum_{i=1}^n \big( bias(\hat{y}|x) \big)^2 
= \sum \beta_2^T \big( x_{1i}^T (X_1^T X_1)^{-1} X_1^T X_2 - x_{2i}^T \big)^T
\big( x_{1i}^T (X_1^T X_1)^{-1} X_1^T X_2 - x_{2i}^T \big) \beta_2$$

$$= \sum \beta_2^T \big( X_2^T X_1 (X_1^T X_1)^{-1} x_{1i} - x_{2i} \big)
\big(x_{1i}^T (X_1^T X_1)^{-1} X_1^T X_2 - x_{2i}^T \big) \beta_2$$

If we FOIL expand the expression: 

$$= \sum \beta_2^T X_2^T \big(X_1 (X_1^T X_1)^{-1} x_{1i}
x_{1i}^T (X_1^T X_1)^{-1} X_1^T \big) X_2 \beta_2
- 2 \sum \beta_2^T X_2^T X_1 (X_1^T X_1)^{-1} x_{1i} x_{2i}^T \beta_2 
+ \sum \beta_2^T x_{2i} x_{2i}^T \beta_2$$

Then using the definition of matrix multiplication: 

$$= \beta_2^T X_2^T X_1 (X_1^T X_1)^{-1} X_1^T X_1 (X_1^T X_1)^{-1} X_1^T X_2 \beta_2
- 2 \beta_2 X_2^T X_1 (X_1^T X_1)^{-1} X_1^T X_2 \beta_2 
+ \beta_2^T X_2^T X_2 \beta_2$$

The first term contains a $(X_1^T X_1)^{-1} (X_1^T X_1)$ which reduces to $I$:

$$= \beta_2^T X_2^T \big( X_1 I (X_1^T X_1)^{-1} X_1^T \big) X_2 \beta_2 
- 2 \beta_2 X_2^T \big( X_1 (X_1^T X_1)^{-1} X_1^T \big) X_2 \beta_2
+ \beta_2^T X_2^T X_2 \beta_2$$

And we can recognize that $H_1 = X_1 (X_1^T X_1)^{-1} X_1^T$:

$$= (X_2 \beta_2)^T H_1 (X_2 \beta_2) - 2 (X_2 \beta_2)^T H_1 (X_2 \beta_2) 
+ (X_2 \beta_2)^T I (X_2 \beta_2)$$

$$= (X_2 \beta_2)^T I (X_2 \beta_2) - (X_2 \beta_2)^T H_1 (X_2 \beta_2)$$

$$= (X_2 \beta_2)^T (I - H_1) (X_2 \beta_2)$$

# Problem 2

## Part a

Recall from S631 that $(H - H_1)$ is symmetric and idempotent. 

*Lemma*: If matrix $A$ is symmetric and idempotent, then it is postiive 
semidefinite

*Proof*: Let $z$ be a nonzero vector. Then since A is symmetric and idempotent,  
$z^T A z = z^T A A z = z^T A^T A z = (Az)^T (Az)$

Define $y = Az$. Then the above is $y^T y \geq 0$. Therefore, $A$ is positive 
semidefinite.

Since $(H - H_1)$ is symmetric and idempotent, it is positive semidefinite.

## Part b