---
title: "STAT-S631"
subtitle: 'Assignment 5'
author: "John Koo"
output: pdf_document
# output: html_document
header-includes:
- \usepackage{float}
---

```{r setup, include = FALSE}
knitr::opts_chunk$set(echo = TRUE, 
                      comment = NA, 
                      fig.pos = 'H', 
                      fig.align = 'center')
options(xtable.comment = FALSE, 
        xtable.table.placement = 'H')
```

# Part a

Start by expanding $(Y - X \hat{\beta})^T (Y - X \hat{\beta})$

$$(Y - X \hat{\beta})^T (Y - X \hat{\beta})$$
$$= Y^T Y - Y^T (X \hat{\beta}) - 
(X \hat{\beta})^T Y + (X \hat{\beta})^T (X \hat{\beta})$$

Note that $x^T y = y^T x$ when $x, y \in \mathbb{R}^n$. So the above is equal to

$$Y^T Y - 2 Y^T (X \hat{\beta}) + (X \hat{\beta})^T (X \hat{\beta})$$

Expanding this out to series:

$$= \sum_i^n y_i^2 - 2 \sum_i^n y_i (x_{i, \cdot} \hat{\beta}) + 
\sum_i^n (x_{i, \cdot} \hat{\beta}) ^ 2$$

$$= \sum_i^n y_i^2 - 2 y_i (x_{i, \cdot} \hat{\beta}) + 
(x_{i, \cdot} \hat{\beta}) ^ 2$$

Which is just an expansion of:

$$ \sum_i^n (y_i - x_{i, \cdot} \hat{\beta}) ^ 2$$

# Part b

If $H$ is symmetric, then $H = H^T$.

$$ H^T = [X(X^T X)^{-1} X^T]^T$$
$$= [X^T]^T [(X^T X)^{-1}]^T [X]^T$$
$$= [X] [(X^T X)^T]^{-1} [X^T]$$
$$= X [(X^T) (X^T)^T]^{-1} X^T$$
$$= X(X^T X)^{-1} X^T$$
$$= H$$
Therefore $H = H^T$.

# Part c

## Show symmetric

$(I - H)^T = I^T - H^T = I - H$

## Show idempotent

We know that $HH = H$.

$(I-H)^2 = II - IH - HI + H^2 = I - H - H + H = I - H$

# Part d

$HX = [X(X^T X)^{-1} X^T] X = X (X^T X)^{-1} (X^T X) = XI = X$

# Part e

$$(I - H)(Y - X \hat{\beta}) = Y - X \hat{\beta} - HY + HX \hat{\beta}$$
$$= Y - X \hat{\beta} - HY + X \hat{\beta}$$
$$= Y - HY = (I - H)Y$$

# Part f

$$(Y - X \hat{\beta})^T (I - H) (Y - X \hat{\beta})$$
$$= [(I - H)^T (Y - X \hat{\beta})]^T (Y - X \hat{\beta})$$
$$= [(I - H)(Y - X \hat{\beta})]^T (Y - X \hat{\beta})$$
$$= [(I - H) Y]^T Y$$
$$= Y^T (I - H)^T Y$$
$$= Y^T (I - H) Y$$

# Part g

$$RSS(\hat{\beta}) = (Y - X \hat{\beta})^T (Y - X \hat{\beta})$$
$$= (Y - HY)^T (Y - HY)$$
$$= Y^T Y - Y^T HY - (HY)^T Y + (HY)^T HY$$
$$= Y^T Y - Y^T HY - Y^T H^T Y + Y^T H^T H Y$$ 
$$= Y^T Y - Y^T H Y - Y^T H Y + Y^T H Y$$
$$= Y^T Y - Y^T H Y$$
$$= (Y^T - Y^T H) Y$$ 
$$= Y^T (I - H) Y$$