---
title: "STAT-S620"
subtitle: 'Assignment 8'
author: "John Koo"
output: pdf_document
# output: html_document
urlcolor: blue
header-includes:
- \usepackage{float}
---

```{r setup, include = FALSE}
knitr::opts_chunk$set(echo = TRUE, 
                      comment = NA, 
                      warning = FALSE, 
                      message = FALSE, 
                      fig.pos = 'H', 
                      fig.align = 'center', 
                      fig.height = 5, 
                      fig.width = 5)
options(xtable.comment = FALSE, 
        xtable.table.placement = 'H')
```

# 5.8.5

$$E[X^r (1 - X)^S] = 
\int_0^1 x^r (1 - x)^s 
\frac{\Gamma(\alpha + \beta)}{\Gamma(\alpha) \Gamma(\beta)}
x^{\alpha - 1} (1 - x)^{\beta - 1} dx$$
$$=\frac{\Gamma(\alpha + \beta)}{\Gamma(\alpha) \Gamma(\beta)} 
\int_0^1 x^{(\alpha + r) - 1} (1 - x)^{(\beta + s) - 1} dx$$
$$= \frac{\Gamma(\alpha + \beta)}{\Gamma(\alpha) \Gamma(\beta)}
\frac{\Gamma(\alpha + r) \Gamma(\beta + s)}{\Gamma(\alpha + r + \beta + s)}$$

# Not from text

## Problem 1

We are given $f(x) = (\theta + 1) x^\theta$ for $x \in [0, 1]$. Then 

$$E[X] = \int_0^1 (\theta + 1) x^{\theta + 1} dx$$
$$= (\theta + 1) \int_0^\infty x^{\theta + 1} dx$$
$$= \frac{\theta + 1}{\theta}$$

Using the method of moments, we set $E[X] = \bar{x}$. Then 

$$\bar{x} = \frac{\hat{\theta} + 1}{\hat{\theta}}$$
$$\hat{\theta} = \frac{1}{\bar{x} - 1}$$

## Problem 2

If $X \sim Gamma(\alpha, \beta)$, then 

$$f(x) = \frac{1}{\Gamma(\alpha) \beta^\alpha} x^{\alpha - 1} e^{-x / \beta}$$
$$= \frac{x^{\alpha - 1}}{\Gamma(\alpha)} \exp({-\alpha \log \beta - x / \beta})$$

Then we can set:

* $\eta(\beta) = 1 / \beta$
* $T(x) = -x$
* $B(\beta) = \alpha \log \beta$

## Part a

We can see from $\eta(\beta)$ that $\beta \neq 0$, and from $B(\beta)$ that 
$\beta > 0$.

## Part b

In order to get the canonical form, we need to replace $B(\beta)$ with 
$A(\eta)$. Since $\eta(\beta) = 1 / \beta$, $\beta = 1 / \eta$. Then 
$A(\eta) = \alpha \log \frac{1}{\eta} = - \alpha \log \eta$. 

$E[T(X)] = E[-X]$, but we also know

$$E[T(X)] = E[-X] = \frac{\partial}{\partial \eta} A(\eta)$$
$$= \frac{\partial}{\partial \eta} (-\alpha \log \eta)$$
$$= -\alpha / \eta$$

$$= -\alpha \beta$$

## Problem 3

We know that $f(\theta | x) \propto f(x | \theta) f(\theta)$. We are also 
given

* $f(x | \theta) = (2 \pi \theta)^{-1/2} \exp(-\frac{(x - \mu)^2}{2 \theta})$
* $f(\theta) = 
\frac{\beta^\alpha}{\Gamma(\alpha)} \theta^{-(\alpha + 1)} e^{-\beta / \theta}$

Then ignoring constant factors,

$$f(\theta | x) \propto \theta^{-1/2} 
\exp \bigg(-\frac{(x - \mu)^2}{2 \theta} \bigg) 
\theta^{-\alpha - 1} \exp(-\beta / \theta)$$
$$\propto \theta^{-(\alpha + \frac{1}{2} + 1)} 
\exp \bigg( -\frac{\frac{(x - \mu)^2}{2} + \beta}{\theta} \bigg)$$

Then we get

$$\theta | x \sim 
InvGamma \bigg(\alpha + \frac{1}{2}, \frac{(x - \mu)^2}{2} + \beta \bigg)$$